Lots of new lemmas, but not much real progress

PermissionLogic.v
@@ -75,7 +75,271 @@ Section DeepPermissions.
 End DeepPermissions.
 
 Set Implicit Arguments.
+
+Require Import List Eqdep_dec.
+
+Definition llist A n := {l : list A | length l = n}.
+
+Lemma ll_proj_eq A n : forall (l l' : llist A n), proj1_sig l = proj1_sig l' -> l = l'.
+ intros.
+ destruct l.
+ destruct l'.
+ simpl in H.
+ subst.
+ f_equal.
+ apply eq_proofs_unicity.
+ decide equality.
+Defined.
+
+  Import Plus.
+
+
+Program Definition llrev A n (l : llist A n) : llist A n := 
+  rev l.
+Obligation 1.
+ destruct l.
+ revert n e.
+ induction x; intros.
+  simpl in *; subst; reflexivity.
+  simpl in *; subst.
+  rewrite app_length.
+  simpl.
+  rewrite (IHx (length x)) by reflexivity.
+  rewrite <- plus_Snm_nSm.
+  rewrite plus_0_r.
+  reflexivity.
+Qed.
+
+Program Definition llcons A n (x : A) (xs : llist A n) : llist A (S n) := cons x xs.
+Obligation 1.
+ destruct xs; subst.
+ reflexivity.
+Qed.
+
+Program Definition llnil A : llist A 0 := nil.
+
+Program Definition llhead A n (l : llist A (S n)) : A :=
+  match l with
+  | nil => _
+  | cons x xs => x
+  end.
+Obligation 1.
+ destruct l.
+ simpl in *.
+ subst; inversion e.
+Qed.
+
+Program Definition lltail A n (l : llist A (S n)) : llist A n :=
+  match l with
+  | nil => _
+  | cons x xs => xs
+  end.
+Obligation 1.
+ destruct l; simpl in *; subst.
+ inversion e.
+Qed.
+Obligation 2.
+  revert l x xs Heq_l.
+  induction n; intuition;
+   destruct l; simpl in *; subst;
+   inversion e; reflexivity.
+Qed.
+
+Program Definition llsnoc A n (l : llist A n) a : llist A (S n) :=
+  l ++ (a :: nil).
+Obligation 1.
+ rewrite app_length.
+ rewrite plus_comm.
+ destruct l.
+ subst; reflexivity.
+Qed.
+
+Program Fixpoint llcohead A n (l : llist A (S n)) : A :=
+  match l with
+  | nil => _
+  | cons x xs => match n with
+     | O => x
+     | S m => llcohead (n:=m) xs end
+  end.
+Obligation 1.
+ destruct l; simpl in *; subst.
+ inversion e.
+Qed.
+Obligation 2.
+ destruct l; simpl in *; subst.
+ inversion e; auto.
+Qed.
+
+
+Program Fixpoint llcotail A n (l : llist A (S n)) : llist A n :=
+  match l with
+  | nil => _
+  | cons x xs => match n with
+    | O => nil
+    | S m => cons x (llcotail (n:=m) xs) end
+  end.
+Next Obligation.
+ destruct l; simpl in *; subst.
+ inversion e.
+Qed.
+Next Obligation.
+ destruct l; simpl in *; subst.
+ inversion e; auto.
+Qed.
+
+
+ 
+
+
+  Hint Resolve ll_proj_eq.
+  Lemma llist_head_tail A n (l : llist A (S n)) : llcons (llhead l) (lltail l) = l.
+   destruct l.
+   destruct x.
+    inversion e.
+    auto with *.
+  Defined.
+
+  Hint Resolve llist_head_tail.
+
+  Lemma llist_ind A : forall P : (forall n, llist A n -> Type),
+    P O (llnil A) ->
+    (forall n l, P n l -> forall a, P (S n) (llcons a l)) ->
+    (forall n l, P n l).
+   intros.
+   induction n.
+    destruct l.
+    destruct x; subst.
+     match goal with |- P 0 ?x => replace x with (llnil A); auto end.
+     inversion e.
+   
+    replace l with (llcons (llhead l) (lltail l)); auto.
+  Defined.    
+
+  Lemma llist_ind0 A : forall P : (llist A 0 -> Type),
+    P (llnil A) -> (forall l, P l).
+   intros.
+   destruct l.
+    destruct x; subst.
+     match goal with |- P ?K => replace K with (llnil A); auto end.
+     inversion e.
+  Defined.
+
+  Lemma llist_indS A : forall P : (forall n, llist A (S n) -> Type),
+    (forall a,  P O (llcons a (llnil A))) ->
+    (forall n l, P n l -> forall a, P (S n) (llcons a l)) ->
+    (forall n l, P n l).
+   intros.
+   induction n.
+    destruct l.
+    destruct x; subst.
+     inversion e.
+     match goal with |- P 0 ?x => replace x with (llcons a (llnil A)); auto end.
+     inversion e.
+      destruct x.
+       auto.
+       inversion H0.
+   
+    replace l with (llcons (llhead l) (lltail l)); auto.
+  Defined.
+
+  Lemma llist_cotail A n a (l : llist A (S n)) :
+      llcotail (llcons a l) = llcons a (llcotail l).
+   revert a.
+   revert n l.
+   refine (llist_indS (fun l => _) _ _); intros.
+    auto.
+    rewrite H.
+    apply ll_proj_eq.
+    simpl.
+    repeat f_equal.
+    apply ll_proj_eq; auto.
+  Qed.
+
+  Lemma llist_cohead A n a (l : llist A (S n)) :
+      llcohead (llcons a l) = llcohead l.
+   destruct l.
+   simpl.
+   f_equal.
+   apply ll_proj_eq.
+   reflexivity.
+  Qed.
+
+  Lemma llist_snoc_cons A n a b (l : llist A n) :
+     llsnoc (llcons a l) b = llcons a (llsnoc l b).
+   revert a b.
+   induction l using llist_ind; intros.
+    auto.
+    auto.
+  Qed.
+
+  Lemma llist_cohead_cotail A n (l : llist A (S n)) :
+     llsnoc (llcotail l) (llcohead l) = l.
+   revert n l;
+   refine (llist_indS (fun l => _) _ _); intros.
+    auto.
+    rewrite llist_cotail.
+    rewrite llist_snoc_cons.
+    f_equal.
+    auto.
+    rewrite llist_cohead.
+    trivial.
+  Qed.
+
+Lemma llist_snoc_ind A : forall P : (forall n, llist A n -> Type),
+    P O (llnil A) ->
+    (forall n l, P n l -> forall a, P (S n) (llsnoc l a)) ->
+    (forall n l, P n l).
+ intros.
+ induction n.
+  destruct l.
+  destruct x; subst.
+   match goal with |- P 0 ?x => replace x with (llnil A); auto end.
+   inversion e.
+
+  rewrite <- llist_cohead_cotail.
+  firstorder.
+Qed.
+
+
+Ltac llniltac := 
+ match goal with L : llist _ 0 |- _ => revert L; refine (llist_ind0 (fun L => _) _) end.
+
+
+
+Lemma ll_snoc_rev_cons A n (l : llist A n) a : llcons a (llrev l) = llrev (llsnoc l a).
+ revert a.
+ induction l using llist_ind.
+  auto.
+
+  intros.
+
+  apply ll_proj_eq.
+  simpl.
+  rewrite app_comm_cons.
+  f_equal.
+  generalize (IHl a0); intro.
+  inversion H.
+  firstorder.
+Qed.
+ 
+
+
+(*
+
+Program Definition myl : llist nat 2 := 1 :: 2 :: nil.
+
+Compute (llsnoc myl 7).
+
+Compute (llhead (lltail myl)).
+
+Compute (proj1_sig (llrev myl)).
+*)
+
+(*
 Set Contextual Implicit Arguments.
+
+
+
 
 Inductive vector (A : Type) : nat -> Type :=
   | vnil : vector A 0
@@ -116,11 +380,113 @@ Program Definition vreverse {A} n (xs : vector A n) : vector A n := vrev xs (@vn
 Compute (vreverse (vcons true (vcons false (vnil bool)))).
 *)
 
+Fixpoint vtol0 A n (v : vector A n) : list A :=
+  match v with
+  | vnil => nil
+  | vcons m x xs => cons x (vtol0 xs)
+  end.
+
+Lemma vtol0_length A n (v : vector A n) : length (vtol0 v) = n.
+ induction v; auto.
+ simpl.
+ f_equal.
+ trivial.
+Defined.
+
+Definition vtol A n (v : vector A n) : {l : list A | length l = n} :=
+  exist _ _ (vtol0_length v).
+
+(*
+Program Fixpoint vtol A n (v : vector A n) : {l : list A & length l = n} :=
+  match v with
+  | vnil => @existT _ _ nil _
+  | vcons m x xs => let (a, b) := vtol xs in @existT  _ _ (cons x a) _
+  end.
+*)
+
+Definition ltov A n (l : {l : list A | length l = n}) : vector A n.
+ induction n.
+  apply vnil.
+  destruct l.
+  destruct x.
+   inversion e.
+   apply vcons.
+   exact a.
+   apply IHn.
+   simpl in e.
+   exists x.
+   injection e; trivial.
+Defined.
+
+Require Import Eqdep_dec.
+
+ 
+
+Lemma ltov_vtol A n (v : vector A n) : ltov (vtol v) = v.
+ induction v.
+  reflexivity.
+  simpl.
+  f_equal.
+  rewrite <- IHv at 8.
+  unfold vtol.
+  f_equal.
+  f_equal.
+  apply eq_proofs_unicity.
+  decide equality.
+Qed.
+
+Lemma length_list_equal A n (l1 l2 : {l : list A | length l = n}) :
+  (let (l1l, _) := l1 in let (l2l, _) := l2 in l1l = l2l) -> l1 = l2.
+intro.
+destruct l1.
+destruct l2.
+subst.
+f_equal.
+apply eq_proofs_unicity.
+decide equality.
+Qed.
+
+Lemma vtol_ltov A n (l : {l : list A | length l = n}) : vtol (ltov l) = l.
+ induction n.
+  destruct l.
+  destruct x.
+   simpl.
+   unfold vtol.
+   f_equal.
+   apply eq_proofs_unicity; decide equality.
+
+   inversion e.
+
+  destruct l.
+  destruct x.
+   inversion e.
+   inversion e.
+   unfold vtol.
+   apply length_list_equal.
+   generalize (IHn (exist _ _ H0)); intro.
+   inversion H.
+   simpl; f_equal.
+   rewrite <- H2 at 3.
+   f_equal.
+   f_equal.
+   f_equal.
+   apply eq_proofs_unicity.
+   decide equality.
+Qed.
+
+Require Import List.
+
+Definition llrev A n (l : {l : list A | length l = n}) : {l : list A | length l = n}
+
+(*
+Compute (vtol (vcons 1 (vnil _) )). *)
+*)
+
 Module InhabitationFunctionDefs.
   Open Scope bool.
-  Definition inhf n := vector bool n -> bool.
+  Definition inhf n := llist bool n -> bool.
   Definition restrict n (f : inhf (S n)) : inhf n :=
-    fun v => f (vcons true v) || f (vcons false v).
+    fun v => f (llcons true v) || f (llcons false v).
   Program Instance inhf_setoid n : Setoid (inhf n) :=
     {| equiv := fun f g => forall v, f v = g v |}.
   Obligation 1.
@@ -135,13 +501,11 @@ Module InhabitationFunctionDefs.
   
 End InhabitationFunctionDefs.
 
-Require Import List.
-
 
 Module Type InhabitationGrid.
   Import InhabitationFunctionDefs.
   Parameter grid : nat -> Type.
-  Parameter eval : forall n, grid n -> vector bool n -> bool.
+  Parameter eval : forall n, grid n -> llist bool n -> bool.
   Parameter empty_grid : grid 0.
   Parameter extensions : forall n, grid n -> list (grid (S n)).
   Axiom empty_grid_is_empty : forall v, eval empty_grid v = true.
@@ -201,7 +565,33 @@ Module TreeInhabitationGrid.
 *)
 
   Definition grid := et.
-  Definition eval' : forall n, grid n -> vector bool n -> bool.
+
+  Program Fixpoint eval' n (g : grid n) (l : llist bool n) : bool :=
+    match g with
+    | et_some => true
+    | et_none m => false
+    | et_branch m L R => match l with
+      | nil => _
+      | cons b bs => if b then eval' R bs else eval' L bs end
+    end.
+  Obligation 1.
+   destruct l.
+   simpl in Heq_l; subst.
+   inversion e.
+  Qed.
+  Obligation 2.
+   destruct l.
+   simpl in *; subst.
+   inversion e; auto.
+  Qed.
+  Obligation 3.
+   destruct l.
+   simpl in *; subst.
+   inversion e; auto.
+  Qed.
+
+(*
+  Definition eval' : forall n, grid n -> llist bool n -> bool.
    fix 1.
    intro.
    destruct n; intros g v.
@@ -210,11 +600,18 @@ Module TreeInhabitationGrid.
      exact false.
     inversion g.
      exact false.
-     inversion v.
-     exact (match H3 with false => eval' n H0 H4 | true => eval' n H1 H4 end).
-  Defined.
-  Definition eval n (g : grid n) (v : vector bool n) :=
-    eval' g (vreverse v).
+     exact (match llhead v with
+         | false => eval' n H0 (lltail v)
+         | true => eval' n H1 (lltail v) end).
+  Defined. *)
+  Definition eval n (g : grid n) (v : llist bool n) :=
+    eval' g (llrev v).
+
+(*
+  Compute (eval (et_branch et_some (et_none 0)) (llcons true (llnil bool))).
+  Compute (eval (et_branch (et_branch et_some (et_some)) (et_none 1)) (llcons true (llcons false (llnil bool)))).
+*)
+
   Definition empty_grid := et_some.
   Proposition empty_grid_is_empty : forall v, eval empty_grid v = true.
    firstorder.
@@ -230,14 +627,71 @@ Module TreeInhabitationGrid.
 
 (*  Compute (extensions (et_branch (et_branch et_some et_some) (et_branch (et_none _) (et_some)))). *)
   
-  Lemma eval_branch n (g1 g2 : grid n) v : eval' (et_branch g1 g1) (vcons true v) = eval' g1 v.
-  reflexivity.
+  Lemma eval_branch n (g1 g2 : grid n) v : eval' (et_branch g1 g1) (llcons true v) = eval' g1 v.
+   simpl.
+   f_equal.
+   apply ll_proj_eq.
+   reflexivity.
   Qed.
-  
+
 
   Proposition extensions_are_extensions : forall n (f : grid (S n)) (g : grid n),
     In f (extensions g) -> is_extension_of (eval f) (eval g).
+   induction n.
+    intros.
+    destruct g; simpl in H; intuition; subst;
+     intro v; try (refine (llist_ind0 (fun v => _) _ v)); try reflexivity.
+     
+     intro v.
+     reflexivity.
+     
+    inversion f.
+   induction f; intros.
+
+(* *)
+
+
    induction g; intros.
+    simpl in H; intuition; subst; intro;
+     refine (llist_ind0 (fun v => _) _ v);
+     reflexivity.
+    simpl in H; intuition; subst; intro.
+     induction v using llist_ind; auto with *.
+
+    simpl in H.
+     apply In_mix_with in H.
+     destruct H; destruct H; intuition; subst.
+     apply IHg1 in H0.
+     apply IHg2 in H.
+     intro.
+     clear -H0 H.
+
+
+     unfold eval in *.
+     unfold is_extension_of in *.
+     unfold restrict in *.
+     replace (llrev v) with (llcons (llhead (llrev v)) (lltail (llrev v))) by auto.
+     simpl.
+
+     unfold eval' at 3.
+     2: apply llist_head_tail.
+     generalize (H0 (lltail v)); intro.
+     simpl in H1.
+     induction v using llist_ind.
+     simpl.
+     unfold eval' at 1.
+     unfold
+  
+     simpl. 
+
+     reflexivity.
+     reflexivity.
+
+
+
+
+
+(* *)
     simpl in H; intuition; subst; intro;
      refine (match v in (vector _ n) with vnil => _ | vcons _ _ _ => id end);
      reflexivity.
@@ -255,6 +709,27 @@ Module TreeInhabitationGrid.
    apply IHg2 in H.
    intro.
    clear -H0 H.
+
+   unfold is_extension_of in H0.
+   unfold eval in *.
+   unfold equiv in H0.
+   unfold inhf_setoid in H0.
+   set (H0 v).
+   simpl in H0.
+   simpl.
+   generalize (vreverse v).
+
+   unfold eval.
+
+   
+
+   refine (match v in (vector _ n0) with vnil => id | _ => _ end).
+   
+   inversion v.
+
+    refine 
+
+
    induction n.
     
     refine (match v in (vector _ n) with vnil => id | vcons _ _ _ => _ end).
